Generalize LiftShift

disj/LiftShift.v
@@ -15,31 +15,59 @@ Reserved Infix "-t>" (at level 50).
 
 (** This typeclass serves as a proof environment for loopsplits **)
 Class disjPaths `(C : redCFG)
-      (q1 q2 s : Lab) (t1 t2 : list (Lab * Tag)) (r1 r2 : list (Lab * Tag)) (j1 j2 k : Tag)
-      (e1 e2 h qs1 qs2 : Lab) (js1 js2 : Tag) :=
+      (q1 q2 s : Lab) (t1 t2 : list (Lab * Tag)) (r1 r2 : list (Lab * Tag)) (j1 j2 k i1 i2 : Tag)
+      (e1 e2 qs1 qs2 : Lab) (js1 js2 : Tag) :=
   {
     Hlc : last_common' t1 t2 r1 r2 (s,k);
-    Hpath1 : TPath (root,start_tag) (q1,j1) t1;
+    Hpath1 : TPath (root,start_tag) (q1,j1) t1
+    where "p --> q" := (edge__P p q);
     Hpath2 : TPath (root,start_tag) (q2,j2) t2
-    where "pi -t> qj" := (tcfg_edge pi qj = true);
+    where "pi -t> qj" := (tcfg_edge pi qj);
+    Hedge1 : (q1,j1) -t> (e1,i1);
+    Hedge2 : (q2,j2) -t> (e2,i2);
+    Hsucc1 : (qs1, js1) ≻ (s, k) | (e1, i1) :: t1;
+    Hsucc2 : (qs2, js2) ≻ (s, k) | (e2, i2) :: t2;
+    Heq12 : eq_loop q1 q2
+  }.
+
+Class disjPathsE `(D : disjPaths) (h : Lab) :=
+  {
     Hexit1 : exit_edge h q1 e1;
     Hexit2 : exit_edge h q2 e2;
-    Hsucc1 : (qs1, js1) ≻ (s, k) | (e1, tl j1) :: t1;
-    Hsucc2 : (qs2, js2) ≻ (s, k) | (e2, tl j2) :: t2;
   }.
+        
 
 Infix "-t>" := tcfg_edge.
 
 
 Lemma disjPaths_sym `(D : disjPaths)
-  : disjPaths C q2 q1 s t2 t1 r2 r1 j2 j1 k e2 e1 h qs2 qs1 js2 js1.
+  : disjPaths C q2 q1 s t2 t1 r2 r1 j2 j1 k i2 i1 e2 e1 qs2 qs1 js2 js1.
 Proof.
   destruct D.
-  econstructor;eauto using last_common'_sym.
+  econstructor;eauto using last_common'_sym. symmetry. eauto.
+Defined.
+
+Lemma disjPaths_sym_iff `(C : redCFG) q1 q2 s t1 t2 r1 r2 j1 j2 k i1 i2 e1 e2 qs1 qs2 js1 js2
+  : disjPaths C q1 q2 s t1 t2 r1 r2 j1 j2 k i1 i2 e1 e2 qs1 qs2 js1 js2
+    <-> disjPaths C q2 q1 s t2 t1 r2 r1 j2 j1 k i2 i1 e2 e1 qs2 qs1 js2 js1.
+Proof.
+  split; intro; eapply disjPaths_sym; eauto.
 Qed.
 
+Lemma disjPathsE_sym `(D : disjPaths) (h : Lab) (D' : disjPathsE D h)
+  : disjPathsE (disjPaths_sym D) h.
+Proof.
+  destruct D'.
+  econstructor;eauto.
+Qed.
 
-Lemma q1_eq_q2 `(D : disjPaths)
+Lemma disjPathsE_sym' `(D : disjPaths) (h : Lab) (D' : disjPathsE (disjPaths_sym D) h)
+  : disjPathsE D h.
+Proof.
+  destruct D. cbn in D'. destruct D'. econstructor;eauto.
+Qed.
+
+Lemma q1_eq_q2 `(D : disjPathsE)
   : eq_loop q1 q2.
 Proof.
   seapply eq_loop_exiting Hexit1 Hexit1'.
@@ -48,9 +76,9 @@ Proof.
   reflexivity. 
 Qed.
 
-Hint Resolve Hlc Hpath1 Hpath2 Hexit1 Hexit2 Hsucc1 Hsucc2 q1_eq_q2 : disjPaths.
+Hint Resolve Hlc Hpath1 Hpath2 Hexit1 Hexit2 Hsucc1 Hsucc2 q1_eq_q2 Heq12 : disjPaths.
 
-Lemma q2_eq_q1 `(D : disjPaths)
+Lemma q2_eq_q1 `(D : disjPathsE)
   : eq_loop q2 q1.
 Proof.
   symmetry. eapply q1_eq_q2;eauto.
@@ -61,14 +89,13 @@ Hint Resolve q2_eq_q1 : disjPaths.
 Class impl_dP
       `(D : disjPaths)
       (q : Lab) (j : Tag)
-      (q1' q2' e1' e2' h' s' : local_impl_CFG_type C q)
+      (q1' q2' e1' e2' s' : local_impl_CFG_type C q)
   :=
     {
       Hq1 : q1 = `q1';
       Hq2 : q2 = `q2';
       He1 : e1 = `e1';
       He2 : e2 = `e2';
-      Hh : h = `h';
       Hocnc : ocnc_loop s q (`s');
       Hndeq : ~ deq_loop q s;
       Hsdeq : deq_loop s q;
@@ -77,30 +104,33 @@ Class impl_dP
     }. 
 
 Lemma impl_dP_sym `(I : impl_dP)
-  : impl_dP (disjPaths_sym D) j q2' q1' e2' e1' h' s'.
+  : impl_dP (disjPaths_sym D) j q2' q1' e2' e1' s'.
 Proof.
   destruct I;econstructor;eauto.
-  - transitivity (`q1');rewrite <-Hq3;eauto. eauto using q1_eq_q2.
+  - transitivity (`q1');rewrite <-Hq3;eauto with disjPaths. 
   - destruct Hjeq0; eauto.
 Qed.
+
+Lemma deq_succ_implode `(C : redCFG) (p q r : Lab)
+      (Hdeq : deq_loop r q)
+      (Hedge : edge__P q p)
+  : implode_nodes C r p.
+Admitted.
 
 Lemma ex_impl_dP1 `(D : disjPaths)
       (Hndeq : ~ deq_loop q1 s)
       (Hsdeq : deq_loop s q1)
-  : exists q1' q2' e1' e2' h' s' : local_impl_CFG_type C q1,
-    impl_dP D j1 q1' q2' e1' e2' h' s'.
+  : exists q1' q2' e1' e2' s' : local_impl_CFG_type C q1,
+    impl_dP D j1 q1' q2' e1' e2' s'.
 Proof.
   assert (implode_nodes C q1 q1).
   { left. reflexivity. }
   assert (implode_nodes C q1 q2). 
   { left. eapply eq_loop2;eauto with disjPaths. reflexivity. }
   assert (implode_nodes C q1 e1).
-  { left. eapply deq_loop_exited. eauto with disjPaths. }
+  { eapply deq_succ_implode. 2: eapply Hedge1. reflexivity. }
   assert (implode_nodes C q1 e2).
-  { left. eapply eq_loop1;[eapply q2_eq_q1;eauto|].
-    eapply deq_loop_exited. eauto with disjPaths. }
-  assert (implode_nodes C q1 h).
-  { left. eapply eq_loop_exiting;eauto with disjPaths. }
+  { eapply deq_succ_implode. 2: eapply Hedge2. destruct D. eapply Heq13. } 
   specialize (ex_ocnc_loop Hndeq Hsdeq) as Hocnc. destructH.
   assert (implode_nodes C q1 s').
   { right. eapply ocnc_loop_exit;eauto. }
@@ -108,11 +138,9 @@ Proof.
   (impl_of_original' H0),
   (impl_of_original' H1),
   (impl_of_original' H2),
-  (impl_of_original' H3),
-  (impl_of_original' H4).
+  (impl_of_original' H3).
   econstructor;cbn;eauto. reflexivity.
 Qed.
-
 
 Definition t1' `{I : impl_dP} := impl_tlist q t1.
 Definition t2' `{I : impl_dP} := impl_tlist q t2.
@@ -136,29 +164,45 @@ Definition qe2 `{I : impl_dP} := fst qej2.
 Definition n1 `{I : impl_dP} := hd 0 (snd qej1).
 Definition n2 `{I : impl_dP} := hd 0 (snd qej2).
 
+Definition h' `{I : impl_dP} := get_innermost_loop' (C := local_impl_CFG C q) q1'.
+
 Section implDP.
 
-  Context `{I : impl_dP}.
+  Context `{I : impl_dP}. 
 
   Lemma lift_disjPaths
-    : disjPaths (local_impl_CFG C q) q1' q2' s' t1' t2' r1' r2' j1 j2 j1 e1' e2' h' qs1' qs2' j1 j1.
+    : disjPaths (local_impl_CFG C q) q1' q2' s' t1' t2' r1' r2' j1 j2 j i1 i2 e1' e2' qs1' qs2' j j.
+  Proof.
+  Admitted.
+
+  Lemma lift_disjPathsE
+    : disjPathsE lift_disjPaths h'.
   Proof.
   Admitted.
 
   Lemma disjPaths_shift_lt
         (Htaglt : n1 < n2)
     : disjPaths C qe1 qe2 s tt1 tt2 rr1 rr2 (n1 :: j) (n2 :: j)
-                k (`qs1') (`qs2') (`s') qs1 qs2 js1 js2.
+                k j j (`qs1') (`qs2') qs1 qs2 js1 js2.
+  Proof.
+  Admitted.
+  
+  Lemma disjPathsE_shift_lt
+        (Htaglt : n1 < n2)
+    : disjPathsE (disjPaths_shift_lt Htaglt) (`s').
   Proof.
   Admitted.
   
   Lemma disjPaths_shift_eq 
         (Htageq : n1 = n2)
-    (*(Hlatchp : CPath (`q2') (`h') (π ++ [`q2']))
-        (Hlatchd : Disjoint (map fst r1) π)*)
-    : (* qs1/2 & js1/2 are turned around because it makes reasoning in the appl. easier*)
-      disjPaths C qe1 qe2 s tt1 tt2 rr1 rr2 (n1 :: j) (n2 :: j)
-                k (`qs1') (`qs2') (`s') qs1 qs2 js1 js2.
+    : disjPaths C qe1 qe2 s tt1 tt2 rr1 rr2 (n1 :: j) (n2 :: j)
+                k j j (`qs1') (`qs2') qs1 qs2 js1 js2.
+  Proof.
+  Admitted.
+
+  Lemma disjPathsE_shift_eq 
+        (Htageq : n1 = n2)
+    : disjPathsE (disjPaths_shift_eq Htageq) (`s').
   Proof.
   Admitted.
   
@@ -191,10 +235,17 @@ Qed.
 Lemma disjPaths_shift_lt2 `(I : impl_dP)
       (Htaglt : n2 < n1)
   : disjPaths C qe1 qe2 s tt1 tt2 rr1 rr2 (n1 :: j) (n2 :: j)
-              k (`qs1') (`qs2') (`s') qs1 qs2 js1 js2.
+              k j j (`qs1') (`qs2') qs1 qs2 js1 js2.
 Proof.
   eapply disjPaths_sym.
   rewrite n1_n2. rewrite n2_n1.
   eapply disjPaths_shift_lt.
   rewrite <-n1_n2. rewrite <-n2_n1. eauto.
-Qed.
+Defined.
+
+Lemma disjPathsE_shift_lt2 `(I : impl_dP)
+      (Htaglt : n2 < n1)
+  : disjPathsE (disjPaths_shift_lt2 Htaglt) (`s').
+Proof.
+  econstructor. admit. admit.
+Admitted.
